$$
\boldsymbol{\tau}_{B}=\left[ \begin{array}{c}{\tau_{\phi}} \\ {\tau_{\theta}} \\ {\tau_{\psi}}\end{array}\right]=
\left[ \begin{array}{c}{l k\left(-\omega_{2}^{2}+\omega_{4}^{2}\right)} \\ {l k\left(-\omega_{1}^{2}+\omega_{3}^{2}\right)} \\ {\sum_{i=1}^{4} (-1)^{i+1} \tau_{M_{i}}}\end{array}\right]
  $$
  $$
  =
\left[ \begin{array}{c}
{k \sum_{i=1}^{4} \omega_{i}^{2}} \\
{l k\left(-\omega_{2}^{2}+\omega_{4}^{2}\right)} \\
{l k\left(-\omega_{1}^{2}+\omega_{3}^{2}\right)} \\
{b(\omega_{1}^{2}-\omega_{2}^{2}+\omega_{3}^{2}-\omega_{4}^{2})}\end{array}\right]
  $$